Clean/Tables/BLAKE3/ProcessBlocksInductive.lean
@@ -81,12 +81,9 @@ def circuit : FormalAssertion (F p) ProcessBlocksState where
   localLength_eq := by
     simp only [circuit_norm, main, U32.AssertNormalized.circuit]
   localAdds_eq _ _ _ := by
-    simp [main, circuit_norm, Operations.collectAdds]
-    constructor
-    · apply Circuit.collectAdds_forEach
-      intro x n; simp [circuit_norm, U32.AssertNormalized.circuit, Operations.collectAdds]
-      rfl
-    · constructor <;> rfl
+    simp only [main, circuit_norm, Operations.collectAdds, List.append_nil]
+    apply Circuit.collectAdds_forEach
+    intro x n; simp only [circuit_norm, Operations.collectAdds]
   subcircuitsConsistent := by
     simp only [circuit_norm, main, U32.AssertNormalized.circuit]
     omega
@@ -147,12 +144,9 @@ def circuit : FormalAssertion (F p) BlockInput where
   localLength_eq := by
     simp only [circuit_norm, main, U32.AssertNormalized.circuit]
   localAdds_eq _ _ _ := by
-    simp [main, circuit_norm, Operations.collectAdds]
-    constructor
-    · rfl
-    · apply Circuit.collectAdds_forEach
-      intro x n; simp [circuit_norm, U32.AssertNormalized.circuit, Operations.collectAdds]
-      rfl
+    simp only [main, circuit_norm, Operations.collectAdds]
+    apply Circuit.collectAdds_forEach
+    intro x n; simp only [circuit_norm, Operations.collectAdds]
   subcircuitsConsistent := by
     simp only [circuit_norm, main, U32.AssertNormalized.circuit]
   Assumptions _ := True
