Clean/Circuit/StructuralLemmas.lean
@@ -38,10 +38,7 @@ def FormalCircuit.concat
       simp only [Circuit.bind_def, Circuit.output, circuit_norm]
     localAdds_eq := by
       intro input env offset
-      simp [Circuit.bind_def, circuit_norm, Operations.collectAdds]
-      constructor
-      · rfl
-      · rfl
+      simp only [Circuit.bind_def, circuit_norm, Operations.collectAdds]
   }
   Assumptions := circuit1.Assumptions
   Spec input output := ∃ mid, circuit1.Spec input mid ∧ circuit2.Spec mid output
