Clean/Gadgets/BLAKE3/FinalStateUpdate.lean
@@ -70,8 +70,7 @@ instance elaborated : ElaboratedCircuit (F p) Inputs BLAKE3State where
   localLength_eq _ n := by
     dsimp only [main, circuit_norm, Xor32.circuit, Xor32.elaborated]
   localAdds_eq _ _ _ := by
-    simp [main, circuit_norm, Operations.collectAdds]
-    and_intros <;> rfl
+    simp only [main, circuit_norm, Operations.collectAdds]
 
 def Assumptions (input : Inputs (F p)) :=
   let { state, chaining_value } := input
