Clean/Gadgets/ByteDecomposition/ByteDecomposition.lean
@@ -46,8 +46,7 @@ def elaborated (offset : Fin 8) : ElaboratedCircuit (F p) field Outputs where
   localLength _ := 2
   output _ i0 := varFromOffset Outputs i0
   localAdds_eq _ _ _ := by
-    simp [circuit_norm, main, Operations.collectAdds]
-    rfl
+    simp only [circuit_norm, main, Operations.collectAdds]
 
 theorem soundness (offset : Fin 8) : Soundness (F p) (circuit := elaborated offset) Assumptions (Spec offset) := by
   intro i0 env x_var (x : F p) h_input (x_byte : x.val < 256) h_holds
